Strata/DL/Imperative/SemanticsProps.lean
@@ -67,3 +67,144 @@ theorem assert_elim
   rw [eval_stmts_singleton] at *
   exact (eval_stmt_assert_eq_of_pure_expr_eq Hwf).mp Heval
 
+theorem UpdateStateComm {P: PureExpr} {x1 x2: P.Ident} {σ σ' σ'' σ1 σ2: SemanticStore P} {v1 v2: P.Expr}
+  [DecidableEq P.Ident]:
+  ¬ x1 = x2 →
+  UpdateState P σ x1 v1 σ1 →
+  UpdateState P σ1 x2 v2 σ' →
+  UpdateState P σ x2 v2 σ2 →
+  UpdateState P σ2 x1 v1 σ'' →
+  σ' = σ'' := by
+  intro Hneq Hu1 Hu2 Hu3 Hu4
+  cases Hu1; cases Hu2; cases Hu3; cases Hu4
+  ext i e
+  rename_i Hfa1 _ _ _ Hfa2 _ _ _ Hfa3 _ _ _ Hfa4 _
+  simp at Hfa1 Hfa2 Hfa3 Hfa4
+  rw[Eq.comm] at Hneq
+  by_cases Heq1: x1 = i
+  simp_all
+  by_cases Heq2: x2 = i
+  rw[Eq.comm] at Hneq
+  specialize Hfa4 x2 Hneq
+  simp_all
+  specialize Hfa1 i Heq1
+  specialize Hfa2 i Heq2
+  specialize Hfa3 i Heq2
+  specialize Hfa4 i Heq1
+  simp_all
+
+theorem UpdateState_InitStateComm {P: PureExpr} {x1 x2: P.Ident} {σ σ' σ'' σ1 σ2: SemanticStore P} {v1 v2: P.Expr}
+  [DecidableEq P.Ident]:
+  ¬ x1 = x2 →
+  UpdateState P σ x1 v1 σ1 →
+  InitState P σ1 x2 v2 σ' →
+  InitState P σ x2 v2 σ2 →
+  UpdateState P σ2 x1 v1 σ'' →
+  σ' = σ'' := by
+  intro Hneq Hu1 Hu2 Hu3 Hu4
+  cases Hu1; cases Hu2; cases Hu3; cases Hu4
+  ext i e
+  rename_i Hfa1 _ _ Hfa2 _ _ Hfa3 _ _ _ Hfa4 _
+  simp at Hfa1 Hfa2 Hfa3 Hfa4
+  rw[Eq.comm] at Hneq
+  by_cases Heq1: x1 = i
+  simp_all
+  by_cases Heq2: x2 = i
+  rw[Eq.comm] at Hneq
+  specialize Hfa4 x2 Hneq
+  simp_all
+  specialize Hfa1 i Heq1
+  specialize Hfa2 i Heq2
+  specialize Hfa3 i Heq2
+  specialize Hfa4 i Heq1
+  simp_all
+
+theorem semantic_eval_eq_of_eval_cmd_set_unrelated_var
+  [HasVarsImp P (Cmd P)] [HasVarsPure P P.Expr]
+  [HasFvar P] [HasVal P] [HasBool P] [HasBoolNeg P]:
+  WellFormedSemanticEvalExprCongr δ →
+  ¬ v ∈ HasVarsPure.getVars e →
+  EvalCmd P δ δP σ₀ σ (Cmd.set v e') σ' →
+  δ σ₀ σ e = δ σ₀ σ' e := by
+  intro Hwf Hnin Heval
+  unfold WellFormedSemanticEvalExprCongr at Hwf
+  specialize Hwf e σ₀ σ σ'
+  have: ∀ (v : P.Ident), v ∈ HasVarsPure.getVars e → σ v = σ' v := by
+    cases Heval
+    rename_i Hu
+    cases Hu
+    rename_i Hfa _
+    intro v' Hv'
+    ext e'
+    by_cases Hc: ¬ v = v'
+    specialize Hfa v' Hc
+    simp_all
+    simp_all
+  exact Hwf this
+
+theorem eval_cmd_set_comm'
+  [HasVarsImp P (List (Stmt P (Cmd P)))] [HasVarsImp P (Cmd P)]
+  [HasFvar P] [HasVal P] [HasBool P] [HasBoolNeg P] [DecidableEq P.Ident] :
+  ¬ x1 = x2 →
+  δ σ₀ σ v1 = δ σ₀ σ2 v1 →
+  δ σ₀ σ v2 = δ σ₀ σ1 v2 →
+  EvalCmd P δ δP σ₀ σ (Cmd.set x1 v1) σ1 →
+  EvalCmd P δ δP σ₀ σ1 (Cmd.set x2 v2) σ' →
+  EvalCmd P δ δP σ₀ σ (Cmd.set x2 v2) σ2 →
+  EvalCmd P δ δP σ₀ σ2 (Cmd.set x1 v1) σ'' →
+  σ' = σ'' := by
+  intro Hneq Heq1 Heq2 Hs1 Hs2 Hs3 Hs4
+  cases Hs1; cases Hs2; cases Hs3; cases Hs4
+  rename_i Hu1 _ _ _ Hu2 _ _ _ Hu3 _ _ _ Hu4
+  simp_all
+  exact UpdateStateComm Hneq Hu1 Hu2 Hu3 Hu4
+
+theorem eval_cmd_set_comm
+  [HasVarsImp P (List (Stmt P (Cmd P)))] [HasVarsImp P (Cmd P)] [HasVarsPure P P.Expr]
+  [HasFvar P] [HasVal P] [HasBool P] [HasBoolNeg P] [DecidableEq P.Ident]:
+  WellFormedSemanticEvalExprCongr δ →
+  ¬ x1 = x2 →
+  ¬ x1 ∈ HasVarsPure.getVars v2 →
+  ¬ x2 ∈ HasVarsPure.getVars v1 →
+  EvalCmd P δ δP σ₀ σ (Cmd.set x1 v1) σ1 →
+  EvalCmd P δ δP σ₀ σ1 (Cmd.set x2 v2) σ' →
+  EvalCmd P δ δP σ₀ σ (Cmd.set x2 v2) σ2 →
+  EvalCmd P δ δP σ₀ σ2 (Cmd.set x1 v1) σ'' →
+  σ' = σ'' := by
+  intro Hwf Hneq Hnin1 Hnin2 Hs1 Hs2 Hs3 Hs4
+  have Heval2:= semantic_eval_eq_of_eval_cmd_set_unrelated_var Hwf Hnin1 Hs1
+  have Heval1:= semantic_eval_eq_of_eval_cmd_set_unrelated_var Hwf Hnin2 Hs3
+  exact eval_cmd_set_comm' Hneq Heval1 Heval2 Hs1 Hs2 Hs3 Hs4
+
+theorem eval_stmt_set_comm
+  [HasVarsImp P (List (Stmt P (Cmd P)))] [HasVarsImp P (Cmd P)] [HasVarsPure P P.Expr]
+  [HasFvar P] [HasVal P] [HasBool P] [HasBoolNeg P] [DecidableEq P.Ident]:
+  WellFormedSemanticEvalExprCongr δ →
+  ¬ x1 = x2 →
+  ¬ x1 ∈ HasVarsPure.getVars v2 →
+  ¬ x2 ∈ HasVarsPure.getVars v1 →
+  EvalStmt P (Cmd P) (EvalCmd P) δ δP σ₀ σ (.cmd (Cmd.set x1 v1)) σ1 →
+  EvalStmt P (Cmd P) (EvalCmd P) δ δP σ₀ σ1 (.cmd (Cmd.set x2 v2)) σ' →
+  EvalStmt P (Cmd P) (EvalCmd P) δ δP σ₀ σ (.cmd (Cmd.set x2 v2)) σ2 →
+  EvalStmt P (Cmd P) (EvalCmd P) δ δP σ₀ σ2 (.cmd (Cmd.set x1 v1)) σ'' →
+  σ' = σ'' := by
+  intro Hwf Hneq Hnin1 Hnin2 Hs1 Hs2 Hs3 Hs4
+  cases Hs1; cases Hs2; cases Hs3; cases Hs4
+  rename_i Hs1 _ Hs2 _ Hs3 _ Hs4
+  exact eval_cmd_set_comm Hwf Hneq Hnin1 Hnin2 Hs1 Hs2 Hs3 Hs4
+
+theorem eval_stmts_set_comm
+  [HasVarsImp P (List (Stmt P (Cmd P)))] [HasVarsImp P (Cmd P)] [HasVarsPure P P.Expr]
+  [HasFvar P] [HasVal P] [HasBool P] [HasBoolNeg P] [DecidableEq P.Ident] :
+  WellFormedSemanticEvalExprCongr δ →
+  ¬ x1 = x2 →
+  ¬ x1 ∈ HasVarsPure.getVars v2 →
+  ¬ x2 ∈ HasVarsPure.getVars v1 →
+  EvalStmts P (Cmd P) (EvalCmd P) δ δP σ₀ σ [(.cmd (Cmd.set x1 v1)), (.cmd (Cmd.set x2 v2))] σ' →
+  EvalStmts P (Cmd P) (EvalCmd P) δ δP σ₀ σ [(.cmd (Cmd.set x2 v2)), (.cmd (Cmd.set x1 v1))] σ'' →
+  σ' = σ'' := by
+  intro Hwf Hneq Hnin1 Hnin2 Hss1 Hss2
+  cases Hss1; cases Hss2
+  rw[eval_stmts_singleton] at *
+  rename_i Hs1 Hs2 _ Hs3 Hs4
+  exact eval_stmt_set_comm Hwf Hneq Hnin1 Hnin2 Hs1 Hs2 Hs3 Hs4
